An version of the interpreter with functions as environments; supports fixpoints in the language

EvalE.v
@@ -2,7 +2,14 @@ Require Import String.
 Require Import List.
 Require Import Ast.
 
+(* TODO: we use definition of monads from Template Coq,
+   but (as actually comment in the [monad_utils] says, we
+   should use a real monad library. )*)
+Require Import Template.monad_utils.
+
+
 Import ListNotations.
+Import MonadNotation.
 
 Module Interpreter.
 
@@ -19,7 +26,9 @@ Module Interpreter.
 
   Inductive val : Type :=
   | vConstr : inductive -> name -> list val -> val
-  | vClos   : env val -> name -> type -> expr -> val.
+  | vClos   : env val -> name ->
+              type (*types are used to convert closures back to lambdas *) ->
+              expr -> val.
 
   (* This doesn't work for the same reason as for STLC: in the case
      for application we don't know if [b] is decreasing.
@@ -62,9 +71,18 @@ Module Interpreter.
   | NotEnoughFuel : res A
   | EvalError : string -> res A.
 
+
   Arguments Ok {_}.
   Arguments NotEnoughFuel {_}.
   Arguments EvalError {_}.
+
+  Instance res_monad : Monad res :=
+    { ret := @Ok;
+      bind := fun _ _ r f => match r with
+                      | Ok v => f v
+                      | EvalError msg => EvalError msg
+                      | NotEnoughFuel => NotEnoughFuel
+                      end }.
 
   Definition option_to_res {A : Type} (o : option A) (msg : string) :=
     match o with
@@ -72,7 +90,7 @@ Module Interpreter.
     | None => EvalError msg
     end.
 
-  Definition todo := EvalError (A:=val) "Not implemented".
+  Definition todo {A} := EvalError (A:=A) "Not implemented".
 
   Definition ind_name (v : val) :=
     match v with
@@ -81,7 +99,7 @@ Module Interpreter.
     end.
 
   (* FIXME: should be extended to match the arguments of the constructor *)
-  Fixpoint match_pat (constr_name : name) (constr_args : list val) (bs : list (pat * expr)) :=
+  Fixpoint match_pat {A} (constr_name : name) (constr_args : list A) (bs : list (pat * expr)) :=
     match bs with
     | [] => None
     | (p, e) :: bs' => if (andb (p.(pName) =? constr_name))
@@ -110,9 +128,9 @@ Module Interpreter.
           | err => err
           end
         | Ok (vConstr ind n vs), Ok v => Ok (vConstr ind n (List.app vs [v]))
-        | EvalError msg, Ok _ => EvalError msg
-        | Ok _, EvalError msg => EvalError msg
-        | _,_ => EvalError "Error in App "
+        | EvalError msg, _ => EvalError msg
+        | _, EvalError msg => EvalError msg
+        | NotEnoughFuel,_ | _, NotEnoughFuel => NotEnoughFuel
         end
       | eConstr t i =>
         Ok (vConstr t i [])
@@ -125,10 +143,130 @@ Module Interpreter.
                                       | None => EvalError "No such constructor"
                                       end
                                     else EvalError ("Expecting inductive " ++ ind ++
-                                                     "but found " ++ ind')
-        | _ => EvalError "Error in Case"
+                                                     " but found " ++ ind')
+        | v => v
         end
-      | eFix nm v ty1 ty2 b => todo
+      | eFix fixname vn ty1 ty2 b as e =>
+        let lam := eLambda vn ty1 b in
+        (* ρ below should be be extended recursively as well :( *)
+        match (expr_eval n Σ ρ lam) with
+        | Ok v' => Ok (vClos (ρ # [fixname ~> v']) vn ty1 b )
+        | e => e
+        end
+         (* expr_eval n Σ (ρ # [fixname ~> vClos ρ fixname (tyArr ty1 ty2) e ]) b *)
+      end
+    end.
+
+  Definition fun_env A := name -> A.
+  Inductive fval : Type :=
+  | fvConstr : inductive -> name -> list fval -> fval
+  | fvClos   : fun_env fval -> name ->
+              type (*types are used to convert closures back to lambdas *) ->
+              expr -> fval.
+
+  Definition ext_env (ρ : fun_env fval) (k : name) v := fun k' => if (string_dec k k') then v else ρ k'.
+  Fixpoint ext_env_list (ρ : fun_env fval) (kvs : list (name * fval)) :=
+    match kvs with
+    | [] => ρ
+    | (k,v) :: kvs' => ext_env (ext_env_list ρ kvs' ) k v
+    end.
+
+
+  Definition default_fun_env : fun_env fval := fun _ => fvConstr "Error" "Error" [].
+  Definition pfun_env A := name -> res A.
+
+  Definition penv_to_total ρ : fun_env fval :=
+    fun k =>
+    match ρ k with
+    | Ok v => v
+    | EvalError msg => fvConstr msg "Error" []
+    | NotEnoughFuel => fvConstr "Not enough fuel" "Error" []
+    end.
+
+  Definition ext_env_rec (fixname : name) (var : name) (ty : type) (e : expr)
+             (ρ : fun_env fval) :=
+    fix rec_enc fuel : res (pfun_env fval) :=
+        match fuel with
+        | O => NotEnoughFuel
+        | S n => Ok (fun k =>
+                      if (eqb fixname k) then
+                        match rec_enc n with
+                          (* FIXME: [penv_to_total] is a hack*)
+                        | Ok ρ' => Ok (fvClos (penv_to_total ρ') var ty e)
+                        | EvalError msg => EvalError msg
+                        | NotEnoughFuel => NotEnoughFuel
+                        end
+                      else Ok (ρ k))
+        end.
+
+  (* This is a simple fact, but it shows that we have two sources of partiality:
+     possible non-termination of the recursive xontext extension and a corresoinding
+     lookup operation (here it is just a function application, but it retirnes a
+     value of type [res fvar] instead of plain [fvar] ) *)
+  Lemma ext_env_rec_extend_lookup : forall n nm vn ty e ρ ρ',
+      ext_env_rec nm vn ty e (penv_to_total ρ) n = Ok ρ ->
+      ρ nm = Ok ρ' ->
+    exists ρ'', ρ' = fvClos ρ'' vn ty e.
+  Proof.
+    intros n nm nv ty e ρ ρ' H1 H2. destruct n.
+    + inversion H1.
+    + destruct n.
+      * inversion H1 as [H3]. rewrite <- H3 in H2. rewrite eqb_refl in H2.
+        inversion H2.
+      * inversion H1 as [H3]. simpl in *.
+        rewrite <- H3 in H2.
+        rewrite eqb_refl in H2.
+        eexists.
+        inversion_clear H2. f_equal.
+  Qed.
+
+  Import Basics.
+
+  Open Scope program_scope.
+
+  Fixpoint expr_eval_fun (fuel : nat) (Σ : global_env) (ρ : fun_env fval) (e : expr) : res fval :=
+    match fuel with
+    | O => NotEnoughFuel
+    | S n =>
+      match e with
+      | eRel i => EvalError "Indices as variables are not supported"
+      | eVar nm => Ok (ρ nm)
+      | eLambda nm ty b =>
+        Ok (fvClos ρ nm ty b)
+      | eLetIn nm e1 ty e2 => todo
+      | eApp e1 e2 =>
+        match (expr_eval_fun n Σ ρ e1), (expr_eval_fun n Σ ρ e2) with
+        | Ok (fvClos ρ' nm _ b), Ok v =>
+          match (expr_eval_fun n Σ (ext_env ρ' nm v) b) with
+          | Ok v' => Ok v'
+          | err => err
+          end
+        | Ok (fvConstr ind n vs), Ok v => Ok (fvConstr ind n (List.app vs [v]))
+        | EvalError msg, _ => EvalError msg
+        | _, EvalError msg => EvalError msg
+        | NotEnoughFuel,_ | _, NotEnoughFuel => NotEnoughFuel
+        end
+      | eConstr t i =>
+        Ok (fvConstr t i [])
+      | eConst nm => todo
+      | eCase (ind,i) ty e bs =>
+        match (expr_eval_fun n Σ ρ e) with
+        | Ok (fvConstr ind' c vs) => if (string_dec ind ind') then
+                                      match (match_pat c vs bs) with
+                                      | Some (var_assign, v) =>
+                                        expr_eval_fun n Σ (ext_env_list ρ var_assign) v
+                                      | None => EvalError "No such constructor"
+                                      end
+                                    else EvalError ("Expecting inductive " ++ ind ++
+                                                     " but found " ++ ind')
+        | v => v
+        end
+      | eFix fixname vn ty1 ty2 e =>
+        match (ext_env_rec fixname vn ty1 e ρ n) with
+        | Ok ρ' => expr_eval_fun n Σ (penv_to_total ρ') (eLambda vn ty1 e)
+        | EvalError msg => EvalError msg
+        | NotEnoughFuel => NotEnoughFuel
+        end
       end
     end.
 
